VRF/Hacl.VRF.DecodeProof.fst
@@ -1,0 +1,41 @@
+module Hacl.VRF.DecodeProof
+
+open FStar.Mul
+
+open FStar.HyperStack
+open FStar.HyperStack.ST
+module ST = FStar.HyperStack.ST
+
+open Spec.Lib
+open Spec.Lib.IntSeq
+
+open Spec.Lib.IntTypes
+open Spec.Lib.IntBuf
+open Spec.Lib.IntBuf.Lemmas
+
+open Hacl.VRF.HashToCurveFinal
+open Hacl.VRF.HashPoints
+
+open Hacl.VRF.Lib
+
+#reset-options " --z3rlimit 100"
+
+val decodeProof: gamma: point -> 
+	c: lbuffer uint8 16 -> s: lbuffer uint8 32 -> 
+	proof: lbuffer uint8 80 -> 
+	Stack bool 
+		(requires  (fun h0 -> live h0 proof /\ live h0 c /\ live h0 s /\ live h0 gamma))
+		(ensures (fun h0 _ h1 -> preserves_live h0 h1 /\ modifies3 gamma c s h0 h1))
+
+let decodeProof gamma c s proof = 
+	let gamma' = sub proof (size 0) (size 32) in 
+	let c' = sub proof (size 32) (size 16) in 
+	let s' = sub proof (size 48) (size 32) in 
+	let valid = decompress gamma gamma' in 
+	if not valid then false else 
+	begin
+		copy (size 16) c' c;
+		copy (size 32) s' s;
+		true
+	end
+	
