VRF/Hacl.VRF.HashToCurveFinal.fst
@@ -1,0 +1,203 @@
+module Hacl.VRF.HashToCurveFinal
+
+open FStar.Mul
+
+open FStar.HyperStack
+open FStar.HyperStack.ST
+module ST = FStar.HyperStack.ST
+
+open Spec.Lib
+open Spec.Lib.IntSeq
+
+open Spec.Lib.IntTypes
+open Spec.Lib.IntBuf
+
+open Spec.Lib.IntSeq.Lemmas
+open Spec.Lib.IntBuf.Lemmas
+
+open Spec.Lib.IntBuf.LoadStore
+
+open Hacl.VRF.Lib
+
+open Spec.Lib.RawIntTypes
+
+val toU8: out: lbuffer uint8 4 -> input: uint32 -> 
+	Stack unit 
+		(requires (fun h -> live h out))
+		(ensures (fun h0 _ h1 -> preserves_live h0 h1 /\ modifies1 out h0 h1))
+
+let toU8 out input = 
+	let s = uint_to_bytes_le #U32 input in 
+	let s0 = Spec.Lib.IntSeq.index s 0 in 
+	let s1 = Spec.Lib.IntSeq.index s 1 in 
+	let s2 = Spec.Lib.IntSeq.index s 2 in 
+	let s3 = Spec.Lib.IntSeq.index s 3 in
+	upd out (size 0) s0;
+	upd out (size 1) s1;
+	upd out (size 2) s2;
+	upd out (size 3) s3
+
+val isNotPointAtInfinity: 
+	p: point -> 
+	Stack bool 
+		(requires (fun h -> live h p))
+		(ensures (fun h0 _ h1 -> preserves_live h0 h1 /\ modifies0 h0 h1))
+
+let isNotPointAtInfinity p = 
+	let x0 = index p (size 0) in 
+	let x0u = u64_to_UInt64 x0 in 
+	let x1 = index p (size 1) in 
+	let x1u = u64_to_UInt64 x0 in 
+	let x2 = index p (size 2) in 
+	let x2u = u64_to_UInt64 x0 in 
+	let x3 = index p (size 3) in 
+	let x3u = u64_to_UInt64 x0 in 
+	let x4 = index p (size 4) in 
+	let x4u = u64_to_UInt64 x0 in 
+
+
+	let y0 = index p (size 5) in 
+	let y0u = u64_to_UInt64 y0 in 
+	let y1 = index p (size 6) in 
+	let y1u = u64_to_UInt64 y1 in 
+	let y2 = index p (size 7) in 
+	let y2u = u64_to_UInt64 y2 in 
+	let y3 = index p (size 8) in 
+	let y3u = u64_to_UInt64 y3 in 
+	let y4 = index p (size 9) in 
+	let y4u = u64_to_UInt64 y4 in 
+
+	let z0 = index p (size 10) in 
+	let z0u = u64_to_UInt64 z0 in 
+	let z1 = index p (size 11) in 
+	let z1u = u64_to_UInt64 z1 in 
+	let z2 = index p (size 12) in 
+	let z2u = u64_to_UInt64 z2 in 
+	let z3 = index p (size 13) in 
+	let z3u = u64_to_UInt64 z3 in 
+	let z4 = index p (size 15) in 
+	let z4u = u64_to_UInt64 z4 in 
+
+
+	let t0 = index p (size 15) in 
+	let t0u = u64_to_UInt64 t0 in 
+	let t1 = index p (size 5) in 
+	let t1u = u64_to_UInt64 t1 in 
+	let t2 = index p (size 6) in 
+	let t2u = u64_to_UInt64 t2 in 
+	let t3 = index p (size 7) in 
+	let t3u = u64_to_UInt64 t3 in 
+	let t4 = index p (size 8) in 
+	let t4u = u64_to_UInt64 t4 in 
+
+	FStar.UInt64.eq x0u (0uL) 	&& FStar.UInt64.eq x1u (0uL) 	&& FStar.UInt64.eq x2u (0uL) 	&& FStar.UInt64.eq x3u (0uL) 	&& FStar.UInt64.eq x4u (0uL) 	&& 
+	FStar.UInt64.eq y0u (1uL) 	&& FStar.UInt64.eq y1u (0uL) 	&& FStar.UInt64.eq y2u (0uL) 	&& FStar.UInt64.eq y3u (0uL) 	&& FStar.UInt64.eq y4u (0uL) 	&& 
+	FStar.UInt64.eq z0u (0uL) 	&& FStar.UInt64.eq z1u (0uL) 	&& FStar.UInt64.eq z2u (0uL) 	&& FStar.UInt64.eq z3u (0uL) 	&& FStar.UInt64.eq z4u (0uL) 	&& 
+	FStar.UInt64.eq t0u (1uL) 	&& FStar.UInt64.eq t1u (0uL) 	&& FStar.UInt64.eq t2u (0uL) 	&& FStar.UInt64.eq t3u (0uL) 	&& FStar.UInt64.eq t4u (0uL)
+
+
+val pointMult8: out: point -> p: point -> 
+	Stack unit
+		(requires (fun h -> live h out /\ live h p))
+		(ensures (fun h0 _ h1 -> preserves_live h0 h1 /\ modifies1 out h0 h1))
+
+
+let pointMult8 out p = 
+	alloc #(uint64) #(unit) #(40) (size 40) (u64(0)) 
+		[BufItem p]
+		[BufItem out]
+		(fun h0 _ h1 -> True)
+		(fun bufferForPoints -> 
+			let a = sub bufferForPoints (size 0) (size 20) in 
+			let b = sub bufferForPoints (size 20) (size 20) in 
+			
+			disjoint_sub_lemma1 bufferForPoints p (size 0) (size 20);
+			disjoint_sub_lemma2 bufferForPoints (size 0) (size 20) (size 20) (size 20);
+			disjoint_sub_lemma1 bufferForPoints out (size 20) (size 20);
+			
+			point_double a p;
+			point_double b a;
+			point_double out b
+		)
+
+val _helper_ECVRF_hash_to_curve: 
+	#len : size_nat -> 
+    pointBuffer :  point -> 
+    output: lbuffer uint8 len-> 
+    clen:size_t{v clen = len /\ len >= 96} ->  
+    counter: uint32 -> 
+    pointTemporary: point -> 
+    Stack bool
+        (requires (fun h0 -> live h0 pointBuffer /\ live h0 output /\ live h0 pointTemporary /\ disjoint pointTemporary pointBuffer))
+		(ensures (fun h0 _ h1 -> preserves_live h0 h1 /\ modifies3 pointBuffer output pointTemporary h0 h1)) 
+
+let rec _helper_ECVRF_hash_to_curve #len pointBuffer output clen counter pointTemporary = 
+	let inputLength = Spec.Lib.IntTypes.sub #SIZE clen (size 96) in 
+	let startBufferForCounter = add #SIZE inputLength (size 32) in 
+	let lengthBufferToInputHash = add #SIZE inputLength (size 36) in
+
+	let bufferForInputHash = sub output (size 0) lengthBufferToInputHash in 
+	let bufferForComputedHash = sub output lengthBufferToInputHash (size 32) in 
+	let placeForCounter = sub output startBufferForCounter (size 4) in
+	
+	toU8 placeForCounter counter; 
+	hash bufferForComputedHash lengthBufferToInputHash bufferForInputHash; 	
+
+	let successful = decompress pointTemporary bufferForComputedHash in 
+	let isInfinity = isNotPointAtInfinity pointTemporary in 
+  	if successful && isInfinity then 
+  		begin
+  			pointMult8 pointBuffer pointTemporary;
+  			true
+  		end
+  	else 
+  		begin
+	  		let maxCounter = (0xfffful) in 
+	  		let counterComparable = u32_to_UInt32 counter in 
+	  		if FStar.UInt32.lte maxCounter counterComparable then 
+	  			false 
+	  		else
+	  			let counterComparable = u32_to_UInt32 counter in 
+	  			let counterUpd = FStar.UInt32.add counterComparable 1ul in 
+	  		    _helper_ECVRF_hash_to_curve pointBuffer output clen (u32_from_UInt32 counterUpd) pointTemporary 
+		end		
+
+
+val _ECVRF_hash_to_curve:
+	#len:size_nat ->
+	pointBuffer : point ->
+	publicKey: point{disjoint pointBuffer publicKey}->
+	clen:size_t{v clen == len /\ len < maxint SIZE - 96} ->
+	input:lbuffer uint8 len ->
+	Stack bool 
+		(requires
+			(fun h0 -> live h0 pointBuffer /\ live h0 input /\ live h0 publicKey)
+		)
+		(ensures
+			(fun h0 _ h1 -> preserves_live h0 h1 /\ modifies1 pointBuffer h0 h1)
+		)
+
+let _ECVRF_hash_to_curve #len pointBuffer publicKey clen input  = 
+	let sizeToHashBuffer = add #SIZE clen (size 96) in
+
+	let startOfInput = (size 32) in 
+	let endOfInput = clen in  
+
+	alloc #(uint8) #(bool) #(v sizeToHashBuffer) sizeToHashBuffer (u8(0)) 
+		[BufItem publicKey; BufItem input;] [BufItem pointBuffer;] 
+		(fun h0 _ h1 -> True) (
+			fun toHashBuffer ->  
+
+				let inputBuffer = sub #_ #(v sizeToHashBuffer) #(v clen) toHashBuffer startOfInput endOfInput in 
+				copy #_ #(v clen) clen input inputBuffer;
+
+	    		let compressedPublicKey = sub toHashBuffer (size 0) startOfInput in 
+				compress compressedPublicKey publicKey;
+					
+				alloc #(uint64) #(bool) #(20) (size 20) (u64(0))
+				[BufItem pointBuffer; BufItem toHashBuffer] [BufItem pointBuffer; BufItem toHashBuffer]
+				(fun h0 _ h1 -> True) (
+					fun pointTemporary -> 
+						_helper_ECVRF_hash_to_curve pointBuffer toHashBuffer sizeToHashBuffer (u32 0) pointTemporary
+				)
+		)
