VRF/Hacl.VRF.ProofToHash.fst
@@ -1,0 +1,62 @@
+module Hacl.VRF.ProofToHash
+
+open FStar.Mul
+
+open FStar.HyperStack
+open FStar.HyperStack.ST
+module ST = FStar.HyperStack.ST
+
+open Spec.Lib
+open Spec.Lib.IntSeq
+
+open Spec.Lib.IntTypes
+open Spec.Lib.IntBuf
+open Spec.Lib.IntBuf.Lemmas
+
+open Hacl.VRF.HashToCurveFinal
+open Hacl.VRF.HashPoints
+
+open Hacl.VRF.Lib
+
+val partialDecodeProof: gamma: point -> 
+	proof: lbuffer uint8 80 -> 
+	Stack bool 
+		(requires  (fun h0 -> live h0 proof /\ live h0 gamma))
+		(ensures (fun h0 _ h1 -> preserves_live h0 h1 /\ modifies1 gamma h0 h1))
+
+let partialDecodeProof gamma proof = 
+	let gamma' = sub proof (size 0) (size 32) in 
+	let valid = decompress gamma gamma' in 
+	if not valid then false else true
+
+val proofToHash:
+	beta: lbuffer uint8 32 ->
+	proof: lbuffer uint8 80 -> 	
+	Stack bool
+		(requires  (fun h0 -> live h0 proof /\ live h0 beta))
+		(ensures (fun h0 _ h1 -> preserves_live h0 h1 /\ modifies1 beta h0 h1))
+			
+let proofToHash beta proof = 
+	alloc #(uint64) #(bool) #(20) (size 20) (u64(0)) 
+		[BufItem proof]
+		[BufItem beta]
+		(fun h0 _ h1 -> True)
+		(fun pointBuffer -> 
+			let r = partialDecodeProof pointBuffer proof in 
+			if not r then false else begin
+			pointMult8 pointBuffer pointBuffer;
+			let sizeHash = size 32 in 
+			alloc #(uint8) #(bool) #(v sizeHash) sizeHash (u8(0))
+				[BufItem pointBuffer]
+				[BufItem beta]
+				(fun h0 _ h1 -> True)
+				(fun bufferForPreHash->
+					let bT = sub  bufferForPreHash (size 0) (size 32) in 
+					compress bT pointBuffer;
+					hash beta (size 32) bufferForPreHash;
+					assert(False);
+					true
+				)
+			end
+		)	
+
